@prefix rdf: <http://www.w3.org/1999/02/22-rdf-syntax-ns#> .
@prefix owl: <http://www.w3.org/2002/07/owl#> .
@prefix rdfs: <http://www.w3.org/2000/01/rdf-schema#> .
@prefix sosa: <http://www.w3.org/ns/sosa/> .
@prefix geosparql: <http://www.opengis.net/ont/geosparql#> .
@prefix xsd: <http://www.w3.org/2001/XMLSchema#> .
@prefix geo: <http://www.w3.org/2003/01/geo/wgs84_pos#> .
@prefix dct: <http://purl.org/dcterms/terms/> .
@prefix skos: <http://www.w3.org/2004/02/skos/core#> .
@prefix ssn: <http://www.w3.org/ns/ssn/> .
@prefix time: <http://www.w3.org/2006/time#> .
@prefix weo: <http://ns.inria.fr/meteo/ontology/> .
@prefix wep: <http://ns.inria.fr/meteo/ontology/property/> .

weo:WeatherStation
  a owl:Class ;
  rdfs:subClassOf sosa:Platform, geosparql:Feature ;
  rdfs:label "Meteo France Synop Weather Station" .

weo:WeatherProperty
  a owl:Class;
  rdfs:label "Weather Property"@en ;
  skos:definition "An observable quality (property, characteristic) of a meterological feature of interest. A weather property can be measured (e.g. wind speed) or observed (cloud cover)."@en ;
  owl:equivalentClass [ owl:intersectionOf (sosa:ObservableProperty
  [ a owl:Restriction ; owl:onProperty ssn:isPropertyOf ; owl:cardinality "1"^^xsd:nonNegativeInteger ]
  [ a owl:Restriction ; owl:onProperty ssn:isPropertyOf ; owl:allValuesFrom weo:MeteorologicalFeature ])] ;
  rdfs:comment "A weather Property is an observable property of exactly one Meterological feature of interest."@en .

weo:MeteorologicalFeature
  a owl:Class, rdfs:Class ;
  rdfs:label "Meteorological Feature"@en;
  skos:definition "The meteorological phenomenon whose property is being measured or observed in the course of an observation."@en ;
  owl:equivalentClass [owl:intersectionOf (sosa:FeatureOfInterest 
  [ a owl:Restriction; owl:onProperty ssn:hasProperty; owl:allValuesFrom weo:WeatherProperty] 
  [ a owl:Restriction; owl:onProperty ssn:hasProperty; owl:minCardinality "1"^^xsd:nonNegativeInteger]) ];
  rdfs:comment "For each Meteorological feature such as wind or precipitations, at least one property (precipitation amount) need to be defined "@en .

weo:MeteorologicalObservation
  a owl:Class ;
  rdfs:label "Meterological Observation"@en ;
  skos:definition "Result of carrying out a procedure to estimate a value of a property of a Meterological feature."@en ;
  owl:equivalentClass [ owl:intersectionOf (sosa:Observation  
  [ a owl:Restriction ; owl:onProperty sosa:observedProperty ; owl:qualifiedCardinality "1"^^xsd:nonNegativeInteger; owl:onClass weo:WeatherProperty]
  [ a owl:Restriction ; owl:onProperty sosa:hasFeatureOfInterest; owl:qualifiedCardinality "1"^^xsd:nonNegativeInteger; owl:onClass weo:MeteorologicalFeature])];
  rdfs:comment " A meterological observation is an observation which is linked to exactly one weather property and one meteorological feature."@en .

weo:Interval3h
    a owl:Class ;
    owl:equivalentClass [ owl:intersectionOf (
        time:Interval
        [   a owl:Restriction;
            owl:onProperty time:hasDuration;
            owl:allValuesFrom  [
                owl:intersectionOf (
                    time:Duration
                    [ a owl:Restriction; owl:onProperty time:numericDuration; owl:hasValue 3.0 ]
                    [ a owl:Restriction; owl:onProperty time:unitType; owl:hasValue time:unitHour]
                )
            ]
        ]    
    )].


weo:Interval6h
    a owl:Class ;
    owl:equivalentClass [ owl:intersectionOf (
        time:Interval
        [   a owl:Restriction;
            owl:onProperty time:hasDuration;
            owl:allValuesFrom  [
                owl:intersectionOf (
                    time:Duration
                    [ a owl:Restriction; owl:onProperty time:numericDuration; owl:hasValue 6.0 ]
                    [ a owl:Restriction; owl:onProperty time:unitType; owl:hasValue time:unitHour]
                )
            ]
        ]    
    )].

weo:Interval12h
    a owl:Class ;
    owl:equivalentClass [ owl:intersectionOf (
        time:Interval
        [   a owl:Restriction;
            owl:onProperty time:hasDuration;
            owl:allValuesFrom  [
                owl:intersectionOf (
                    time:Duration
                    [ a owl:Restriction; owl:onProperty time:numericDuration; owl:hasValue 12.0 ]
                    [ a owl:Restriction; owl:onProperty time:unitType; owl:hasValue time:unitHour]
                )
            ]
        ]    
    )].

weo:Interval24h
    a owl:Class ;
    owl:equivalentClass [ owl:intersectionOf (
        time:Interval
        [   a owl:Restriction;
            owl:onProperty time:hasDuration;
            owl:allValuesFrom  [
                owl:intersectionOf (
                    time:Duration
                    [ a owl:Restriction; owl:onProperty time:numericDuration; owl:hasValue 24.0 ]
                    [ a owl:Restriction; owl:onProperty time:unitType; owl:hasValue time:unitHour]
                )
            ]
        ]    
    )].


weo:Interval10m
    a owl:Class ;
    owl:equivalentClass [ owl:intersectionOf (
        time:Interval
        [   a owl:Restriction;
            owl:onProperty time:hasDuration;
            owl:allValuesFrom  [
                owl:intersectionOf (
                    time:Duration
                    [ a owl:Restriction; owl:onProperty time:numericDuration; owl:hasValue 10.0 ]
                    [ a owl:Restriction; owl:onProperty time:unitType; owl:hasValue time:unitMinute]
                )
            ]
        ]    
    )].

    
wep:madeByStation
  a owl:ObjectProperty ; 
  rdfs:domain <http://ns.inria.fr/meteo/ontology/WeatherStation> ;
  rdfs:range <http://ns.inria.fr/meteo/ontology/MeteorologicalObservation> .
 
wep:stationID
  a owl:DatatypeProperty ;
  skos:prefLabel "ID";
  rdfs:domain <http://ns.inria.fr/meteo/ontology/WeatherStation> .

wep:hasAbbreviation
  a owl:DatatypeProperty ;
  skos:prefLabel "Mn√©monique"@fr;
  rdfs:domain <http://ns.inria.fr/meteo/ontology/WeatherProperty> .
